src/ReactorModel/Determinism/ExecutionStep.lean
@@ -2,6 +2,7 @@ import ReactorModel.Determinism.InstExecution
 
 namespace Execution
 
+open ReactorType 
 open State (Closed)
 
 variable [State.Nontrivial s] [State.Nontrivial s₁]
@@ -36,19 +37,16 @@ theorem not_Closed (e : s₁ ⇓| s₂) : ¬(Closed s₁) := by
   exact e.fresh ▸ State.Nontrivial.nontrivial.ne_empty.symm 
 
 theorem preserves_tag (e : s₁ ⇓| s₂) : s₁.tag = s₂.tag :=
-  e.exec.tag_eq
+  e.exec.preserves_tag
 
-theorem preserves_rcns (e : s₁ ⇓| s₂) : s₁.rtr[.rcn].ids = s₂.rtr[.rcn].ids :=
-  congr_arg _ e.exec.preserves_rcns
-
-theorem rcns_eq (e₁ : s ⇓| s₁) (e₂ : s ⇓| s₂) : s₁.rtr[.rcn].ids = s₂.rtr[.rcn].ids :=
-  e₁.preserves_rcns ▸ e₂.preserves_rcns
+theorem equiv (e : s₁ ⇓| s₂) : s₁.rtr ≈ s₂.rtr :=
+  e.exec.equiv
   
 theorem rcns_Nodup (e : s₁ ⇓| s₂) : e.rcns.Nodup := 
   e.exec.rcns_nodup
 
 theorem progress_def (e : s₁ ⇓| s₂) : s₂.progress = s₁.rtr[.rcn].ids :=
-  e.preserves_rcns ▸ e.closed
+  Equivalent.obj?_rcn_eq e.equiv ▸ e.closed
 
 theorem mem_rcns_iff (e : s₁ ⇓| s₂) : rcn ∈ e.rcns ↔ (rcn ∈ s₁.rtr[.rcn].ids ∧ rcn ∉ s₁.progress) :=
   e.progress_def ▸ e.exec.mem_rcns_iff
@@ -57,7 +55,7 @@ theorem rcns_perm (e₁ : s ⇓| s₁) (e₂ : s ⇓| s₂) : e₁.rcns ~ e₂.r
   simp [List.perm_ext e₁.rcns_Nodup e₂.rcns_Nodup, e₁.mem_rcns_iff, e₂.mem_rcns_iff]
 
 theorem tag_eq (e₁ : s ⇓| s₁) (e₂ : s ⇓| s₂) : s₁.tag = s₂.tag :=
-  e₁.exec.tag_eq ▸ e₂.exec.tag_eq
+  e₁.exec.preserves_tag ▸ e₂.exec.preserves_tag
 
 theorem progress_eq (e₁ : s ⇓| s₁) (e₂ : s ⇓| s₂) : s₁.progress = s₂.progress := by
   simp [e₁.progress_def, e₂.progress_def]
@@ -69,7 +67,7 @@ theorem step_determined (e : s ⇓| s₁) (a : s ⇓- s₂) : False :=
   absurd a.closed e.not_Closed
 
 instance preserves_Nontrivial [h : State.Nontrivial s₁] {e : s₁ ⇓| s₂} : State.Nontrivial s₂ where
-  nontrivial := e.preserves_rcns ▸ h.nontrivial
+  nontrivial := Equivalent.obj?_rcn_eq e.equiv ▸ h.nontrivial
 
 theorem nonrepeatable (e₁ : s₁ ⇓| s₂) (e₂ : s₂ ⇓| s₃) : False :=
   have := e₁.preserves_Nontrivial -- TODO: Make this work via type class inference.
